CC.v
@@ -1,0 +1,122 @@
+Set Implicit Arguments.
+Unset Strict Implicit.
+
+Require Import List.
+Require Import core unscoped hopl translation.
+
+Import RenNotations.
+Import SubstNotations.
+Import CombineNotations.
+Import UnscopedNotations.
+
+Notation lup := nth_error.
+
+
+
+(* Monotonicity *)
+
+Lemma HOPL_AE' A t phi phi' e :
+  HOPL_prv A (tmall t phi) -> phi' = (subst_spec var_type (e..) var_exp) phi -> HOPL_prv A phi'.
+Proof.
+  intros H ->. now apply HOPL_EAE with t.
+Qed.
+
+Lemma int_mono t phi psi m :
+  HOPL_prv (tmall t (spimplies phi psi) :: nil) (spimplies (after m phi) (after m psi)).
+Proof.
+  apply HOPL_II. eapply HOPL_MM. 2: apply HOPL_CTX; now left.
+  eapply HOPL_IE. 2: apply HOPL_CTX; now left.
+  eapply (HOPL_AE' (e := var_prog 0)).
+  - cbn. apply HOPL_CTX. right. right. now left.
+  - asimpl. unfold funcomp. f_equal.
+    + rewrite idSubst_spec; trivial. now intros [].
+    + rewrite idSubst_spec; trivial. now intros [].
+Qed.
+
+
+
+(* Existential *)
+
+Definition exis s phi :=
+  all 1 (implies (all s (implies (ren_form swap phi) (holds (var_term 1) (var_term 2)))) ((holds (var_term 0) (var_term 1)))).
+
+Lemma ip_exis Xi phi s :
+  lup Xi 0 = Some 0 -> is_prop (s :: Xi) phi -> is_prop Xi (exis s phi).
+Proof.
+  intros H1 H2.
+  unfold exis.
+  apply ip_all, ip_implies.
+  - apply ip_all, ip_implies.
+    + eapply is_prop_ren; eauto. now intros [].
+    + apply ip_holds with 0; now apply hs_var.
+  - apply ip_holds with 0; now apply hs_var.
+Qed.
+
+Lemma HOL_AE' A s phi phi' p :
+  HOL_prv A (all s phi) -> phi' = phi[p..] -> HOL_prv A phi'.
+Proof.
+  intros H ->. now apply HOL_AE with s.
+Qed.
+
+Lemma HOL_CE' A p s phi phi' :
+  HOL_prv A (holds (cterm s phi) p) -> phi' = phi[p..] -> HOL_prv A phi'.  
+Proof.
+  intros H ->. now apply HOL_CE with s.
+Qed.
+
+Lemma HOL_eq A phi B psi :
+  HOL_prv A phi -> A = B -> phi = psi -> HOL_prv B psi.
+Proof.
+  intros H -> ->. apply H.
+Qed.
+
+Lemma HOL_ren A phi xi :
+  HOL_prv A phi -> HOL_prv (map (ren_form xi) A) (ren_form xi phi).
+Proof.
+  induction 1 in xi |- * ; cbn in *.
+  - constructor. now apply in_map.
+  - econstructor 2. eauto.
+  - econstructor 3; eauto.
+  - econstructor 4. eapply HOL_eq. 3: reflexivity.
+    + apply IHHOL_prv.
+    + rewrite !map_map. apply map_ext. intros psi. now asimpl.
+  - eapply HOL_eq. 2: reflexivity.
+    + econstructor 5 with (p := p⟨xi⟩). apply IHHOL_prv.
+    + cbn. now asimpl.
+  - econstructor 6. eapply HOL_eq. 2: reflexivity.
+    + apply IHHOL_prv.
+    + now asimpl.
+  - eapply HOL_eq. 2: reflexivity.
+    + econstructor 7. apply IHHOL_prv.
+    + now asimpl.
+Qed.
+
+Lemma HOL_EI A phi s p :
+  HOL_prv A phi[p..] -> HOL_prv A (exis s phi).
+Proof.
+  intros H. unfold exis. apply HOL_AI, HOL_II.
+  apply HOL_IE with (ren_form ↑ (phi[p..])).
+  - eapply (HOL_AE' (p := ren_term ↑ p)).
+    + apply HOL_CTX. now left.
+    + now asimpl.
+  - eapply HOL_weak; try apply HOL_ren; eauto. firstorder.
+Qed.
+
+Lemma HOL_EE A phi psi s :
+  HOL_prv A (exis s phi) -> HOL_prv (phi :: map (ren_form ↑) A) (ren_form ↑ psi) -> HOL_prv A psi.
+Proof.
+  intros H1 H2. unfold exis in H1. apply (HOL_AE (cterm 42 (ren_form swap psi))) in H1.
+  cbn in H1. eapply HOL_CE'.
+  - eapply HOL_IE. 1: try apply H1.
+    apply HOL_AI. asimpl. rewrite idSubst_form; try now intros [].
+    apply HOL_II. apply HOL_CI. asimpl. rewrite rinstInst'_form in H2.
+    erewrite ext_form; try apply H2. now intros [].
+  - unfold swap. asimpl. rewrite idSubst_form; trivial. now intros [].
+Qed.
+
+
+
+(* Countable Choice *)
+
+Definition CC s phi : form :=
+  all s phi.
